progress in RInvoke of canCommit + new invs on disjoint ro/wo

txn-data-consistency/EP+_Invariants.thy
@@ -776,11 +776,8 @@ lemma t_is_fresh:
 
 subsection \<open>Read-Only and Write-Only\<close>
 
-definition Disjoint_RW where
-  "Disjoint_RW s \<longleftrightarrow> ((\<Union>k. wtxns_dom (svr_state (svrs s k))) \<inter> Tn ` (\<Union>k. wtxns_rsran (svr_state (svrs s k))) = {})" (* not proven *)
-
-(*definition Disjoint_RW' where
-  "Disjoint_RW' s \<longleftrightarrow> (kvs_writers (kvs_of_s s) \<inter> Tn ` kvs_readers (kvs_of_s s) = {})"*)
+(*definition Disjoint_RW where
+  "Disjoint_RW s \<longleftrightarrow> ((\<Union>k. wtxns_dom (svr_state (svrs s k))) \<inter> Tn ` (\<Union>k. wtxns_rsran (svr_state (svrs s k))) = {})"*)
 
 definition RO_has_rts where
   "RO_has_rts s \<longleftrightarrow> (\<forall>t. Tn t \<in> read_only_Txs (kvs_of_s s) \<longrightarrow> (\<exists>rts. rtxn_rts s t = Some rts))" (* not proven *)
@@ -973,6 +970,23 @@ definition RO_WO_Inv where
 subsection \<open>Views\<close>
 
 subsubsection \<open>View Invariants\<close>
+
+definition Disjoint_RW where
+  "Disjoint_RW s \<longleftrightarrow> (read_only_Txs (kvs_of_s s) = Tn ` kvs_readers (kvs_of_s s))"
+
+lemma kvs_writers_readers_disjoint:
+  "reach tps_s s \<Longrightarrow> kvs_writers (kvs_of_s s) \<inter> Tn ` kvs_readers (kvs_of_s s) = {}" oops
+
+definition PTid_In_KVS where
+  "PTid_In_KVS s cl \<longleftrightarrow> (case cl_state (cls s cl) of
+    WtxnCommit _ _ \<Rightarrow> (\<forall>n \<le> cl_sn (cls s cl). Tn (Tn_cl n cl) \<in> kvs_txids (kvs_of_s s)) |
+    _ \<Rightarrow> (\<forall>n < cl_sn (cls s cl). Tn (Tn_cl n cl) \<in> kvs_txids (kvs_of_s s)))"
+
+lemma SO_in_kvs_txids:
+  assumes "reach tps_s s"
+    and "Tn (Tn_cl m cl) \<in> kvs_txids (kvs_of_s s)"
+    and "n < m"
+  shows "Tn (Tn_cl n cl) \<in> kvs_txids (kvs_of_s s)" oops
 
 definition View_Closed where
   "View_Closed s cl \<longleftrightarrow> closed' (kvs_of_s s) (\<Union>k. get_view s cl k) (R_CC (kvs_of_s s))" (* not proven *)
